aes/verif_encryption_LL.v
@@ -4,6 +4,7 @@ Require Import aes.encryption_LL_round_step_eqs.
 Require Import aes.verif_encryption_LL_loop_body.
 Require Import aes.verif_encryption_LL_after_loop.
 Open Scope Z.
+Require Import VST.floyd.Funspec_old_Notation.
 
 Lemma body_aes_encrypt: semax_body Vprog Gprog f_mbedtls_aes_encrypt encryption_spec_ll.
 Proof.
