progs/VSUpile/verif_pile.v
@@ -201,8 +201,8 @@ simpl in H0.
  rep_omega.
  f_equal; f_equal; omega.
 apply -> wand_sepcon_adjoint.
-match goal with |- _ * ?A * ?B * ?C |-- _ => 
- assert (A * B * C |-- listrep M (z::s2) r) end.
+match goal with |- (_ * ?A * ?B * ?C)%logic |-- _ => 
+ assert ((A * B * C)%logic |-- listrep M (z::s2) r) end.
 unfold listrep at 2; fold (listrep M). Exists r'. entailer!.
 sep_apply H10.
 sep_apply modus_ponens_wand.
