tweetnacl20140427/verif_crypto_core.v
@@ -4,6 +4,7 @@ Require Import List. Import ListNotations.
 Require Import tweetnacl20140427.Snuffle.
 Require Import tweetnacl20140427.Salsa20.
 Require Import ZArith.
+Local Open Scope Z.
 
 Require Import tweetnacl20140427.tweetnaclVerifiableC.
 Require Import tweetnacl20140427.spec_salsa.
